riscv: add kdev_base/kdevBase to handle RISCVVSpaceDeviceWindow and update proofs
- Add HiFive.hs to replace Spike.hs, it's the same except for kdevBase
  addition.
- Originally called KDEV_PPTR in the C Code, to be changed to KDEV_BASE
  across all architectures.
- Add RISCVVSpaceDeviceWindow case for valid_uses_2 definition.

spec/abstract/RISCV64/Machine_A.thy
@@ -125,6 +125,13 @@ definition user_vtop :: "machine_word"
   "user_vtop = Platform.RISCV64.pptrUserTop"
 
 text \<open>
+  Virtual address for start of kernel device mapping region in highest 1GiB of memory.
+\<close>
+definition kdev_base :: "machine_word"
+  where
+  "kdev_base = Platform.RISCV64.kdevBase"
+
+text \<open>
   The virtual address the kernel code is mapped.
 \<close>
 definition kernel_elf_base :: "vspace_ref"
